finished part of read skip

fstar/StorageToMemory.fst
@@ -1,10 +1,10 @@
 module StorageToMemory
 
+open FStar.List
 open Memory
 open Storage
 
 let rec copyStAux #v #i #a #c (mem : memoryI a v i c)
-
   (id : idIB a v i) (st : structB c v i) : Tot (memoryI a v i c) (decreases %[st; id])
   = match st, id with
   | Mtst, _ -> mem
@@ -15,3 +15,44 @@ let rec copyStAux #v #i #a #c (mem : memoryI a v i c)
 
 let copySt #v #i #a #c (mem : memoryI a v i c) (id : a) (st : structB c v i) : memoryI a v i c =
     copyStAux (Add mem id) (id, []) st
+
+let rec is_same (#a : eqtype) (l1 l2 : list a) : bool
+  = match l1, l2 with
+  | [], [] -> true
+  | x :: xs, y :: ys -> x = y && xs `is_same` ys
+  | _ -> false
+
+let rec is_same_same (#a : eqtype) (l1 l2 : list a) :
+  Lemma (requires is_same l1 l2) (ensures l1 == l2)
+  = match l1, l2 with
+  | [], [] -> _
+  | x :: xs, y :: ys -> is_same_same xs ys
+
+let rec is_same_rev (#a : eqtype) (l : list a) :
+  Lemma (is_same l l)
+  = match l with
+  | [] -> _
+  | _ :: xs -> is_same_rev xs
+
+let rec is_suffix_of (#a : eqtype) (l1 l2 : list a) : bool
+  = l1 `is_same` l2 || (match l2 with
+    | []  -> false
+    | _ :: q -> l1 `is_suffix_of` q
+    )
+
+let suffix_equal (#a : eqtype) (x : a) (l : list a) :
+  Lemma (ensures l `is_suffix_of` (x :: l))
+  = match l with
+  | [] -> _
+  | _ :: xs -> is_same_rev xs
+
+let rec readSkip (#v : eqtype) (#i :eqtype) (#a : eqtype) (mem : memoryI a v i nat) (pId : a)
+  (pIdR : a) (st : structB nat v i) (fxsL : list (either v i)) (fxsR : list (either v i)) (fld : either v i) :
+  Lemma (requires pId <> pIdR || pId = pIdR && not (fxsL `is_suffix_of` (fld :: fxsR)))
+    (ensures read (copyStAux mem (pId, fxsL) st) (pIdR , fxsR) fld == read mem (pIdR , fxsR) fld) =
+    match st with
+    | Mtst -> _
+    | Store st' (Inl f) (Var _) ->
+      readSkip mem pId pIdR st' fxsL fxsR fld;
+      suffix_equal fld fxsL
+    | Store _ (Inr _) _ -> admit()
